src/tlogic/TemporalLogic.v
@@ -1183,27 +1183,27 @@ Section TRIPLE.
   (*      Syntax.striple_format tid I0 I1 I2 P Q E1 E2 (fun rs rt => ⤉ (syn_term_cond n tid R_term rs rt)) ps pt itr_src code ktr_tgt)%S. *)
 
   Definition syn_triple_gen
-             n δ tid (P : sProp (δ + n)) {RV} (Q : RV -> sProp (δ + n)) (E1 E2 : coPset)
-    : forall {R_term : Type}, bool -> bool -> itree srcE R_term -> itree tgtE RV -> ktree tgtE RV R_term -> sProp (δ + n)
+             n δ tid (P : sProp (S (δ + n))) {RV} (Q : RV -> sProp (S (δ + n))) (E1 E2 : coPset)
+    : forall {R_term : Type}, bool -> bool -> itree srcE R_term -> itree tgtE RV -> ktree tgtE RV R_term -> sProp (S (δ + n))
     :=
     fun R_term ps pt itr_src code ktr_tgt =>
-      (let N := (δ + n) in
+      (let N := (S (δ + n)) in
         let I0 := (fun ths ims imt sts stt => ((syn_default_I N ths ims imt sts stt) ∗ (⟨syn_wsat_auth N⟩ ∗ syn_wsats N ∗ ⟨owne ⊤⟩))%S)
        in
        let I1 := (fun ths ims imt sts stt => ((syn_default_I_past tid N ths ims imt sts stt) ∗ (⟨syn_wsat_auth N⟩ ∗ syn_wsats N ∗ ⟨owne ⊤⟩))%S)
        in
        let I2 := (fun ths im_src im_tgt st_src st_tgt E => (syn_default_I_past tid N ths im_src im_tgt st_src st_tgt ∗ (⟨syn_wsat_auth N⟩ ∗ syn_wsats N ∗ ⟨owne E⟩)))
        in
-       Syntax.striple_format tid I0 I1 I2 P Q E1 E2 (fun rs rt => lifts (syn_term_cond n tid R_term rs rt) δ) ps pt itr_src code ktr_tgt)%S.
+       Syntax.striple_format tid I0 I1 I2 P Q E1 E2 (fun rs rt => lifts (syn_term_cond n tid R_term rs rt) (S δ)) ps pt itr_src code ktr_tgt)%S.
 
 
   Lemma red_syn_triple_gen
-        n δ tid (P : sProp (δ + n)) RV (Q : RV -> sProp (δ + n)) E1 E2
+        n δ tid (P : sProp (S (δ + n))) RV (Q : RV -> sProp (S (δ + n))) E1 E2
         R_term ps pt itr_src code (ktr_tgt : ktree tgtE RV R_term)
     :
-    ⟦syn_triple_gen n δ tid P Q E1 E2 ps pt itr_src code ktr_tgt, δ + n⟧
+    ⟦syn_triple_gen n δ tid P Q E1 E2 ps pt itr_src code ktr_tgt, S (δ + n)⟧
     =
-      triple_gen (δ + n) n tid ⟦P, δ + n⟧ (fun rv => ⟦Q rv, δ + n⟧) E1 E2 ps pt itr_src code ktr_tgt.
+      triple_gen (S (δ + n)) n tid ⟦P, S (δ + n)⟧ (fun rv => ⟦Q rv, S (δ + n)⟧) E1 E2 ps pt itr_src code ktr_tgt.
   Proof.
     unfold syn_triple_gen, triple_gen. red_tl. unfold triple_format.
     apply f_equal. extensionalities rr. apply f_equal. extensionalities gr.
@@ -1221,9 +1221,9 @@ Section TRIPLE.
       apply f_equal. extensionalities st_src. apply f_equal. extensionalities st_tgt.
       red_tl. simpl. red_tl. rewrite red_syn_default_I_past. rewrite red_syn_wsats.
       f_equal. f_equal.
-      + symmetry. apply (red_isim_eq_1 (δ + n)).
-      + apply (red_isim_eq_2 _ (δ + n)).
-      + apply (red_isim_eq_2 _ (δ + n)).
+      + symmetry. apply (red_isim_eq_1 (S (δ + n))).
+      + apply (red_isim_eq_2 _ (S (δ + n))).
+      + apply (red_isim_eq_2 _ (S (δ + n))).
       + symmetry.
         extensionalities r_src r_tgt ths1 im_src1 im_tgt1.
         extensionalities st_src1 st_tgt1.
@@ -1235,9 +1235,9 @@ Section TRIPLE.
       apply f_equal. extensionalities st_src. apply f_equal. extensionalities st_tgt.
       red_tl. simpl. red_tl. rewrite red_syn_default_I_past. rewrite red_syn_wsats.
       f_equal. f_equal.
-      + symmetry. apply (red_isim_eq_1 (δ + n)).
-      + apply (red_isim_eq_2 _ (δ + n)).
-      + apply (red_isim_eq_2 _ (δ + n)).
+      + symmetry. apply (red_isim_eq_1 (S (δ + n))).
+      + apply (red_isim_eq_2 _ (S (δ + n))).
+      + apply (red_isim_eq_2 _ (S (δ + n))).
       + symmetry.
         extensionalities r_src r_tgt ths1 im_src1 im_tgt1.
         extensionalities st_src1 st_tgt1.
@@ -1246,22 +1246,22 @@ Section TRIPLE.
 
   Definition syn_atomic_triple
              tid n δ (E : coPset)
-             (P : sProp (δ + n)) {RV} (code : itree tgtE RV) (Q : RV -> sProp (δ + n))
-    : sProp (δ + n)
+             (P : sProp (S (δ + n))) {RV} (code : itree tgtE RV) (Q : RV -> sProp (S (δ + n)))
+    : sProp (S (δ + n))
     :=
     (∀ (R_term : τ{metaT})
        (ps pt : τ{bool})
-       (itr_src : τ{codeT id_src_type st_src_type R_term, δ + n})
-       (ktr_tgt : τ{(RV -> codeT id_tgt_type st_tgt_type R_term)%stype, δ + n}),
+       (itr_src : τ{codeT id_src_type st_src_type R_term, S (δ + n)})
+       (ktr_tgt : τ{(RV -> codeT id_tgt_type st_tgt_type R_term)%stype, S (δ + n)}),
         (syn_triple_gen n δ tid P Q E E ps pt itr_src code ktr_tgt))%S.
 
   Lemma red_syn_atomic_triple
         tid n δ (E : coPset)
-        (P : sProp (δ + n)) RV (code : itree tgtE RV) (Q : RV -> sProp (δ + n))
+        (P : sProp (S (δ + n))) RV (code : itree tgtE RV) (Q : RV -> sProp (S (δ + n)))
     :
-    ⟦syn_atomic_triple tid n δ E P code Q, δ + n⟧
+    ⟦syn_atomic_triple tid n δ E P code Q, S (δ + n)⟧
     =
-      atomic_triple tid (δ + n) n E ⟦P, δ + n⟧ code (fun v => ⟦Q v, δ + n⟧).
+      atomic_triple tid (S (δ + n)) n E ⟦P, S (δ + n)⟧ code (fun v => ⟦Q v, S (δ + n)⟧).
   Proof.
     unfold syn_atomic_triple, atomic_triple. red_tl.
     apply f_equal. extensionalities R_term. red_tl.
@@ -1274,22 +1274,22 @@ Section TRIPLE.
 
   Definition syn_non_atomic_triple
              tid n δ (E : coPset)
-             (P : sProp (δ + n)) {RV} (code : itree tgtE RV) (Q : RV -> sProp (δ + n))
-    : sProp (δ + n)
+             (P : sProp (S (δ + n))) {RV} (code : itree tgtE RV) (Q : RV -> sProp (S (δ + n)))
+    : sProp (S (δ + n))
     :=
     (∀ (R_term : τ{metaT})
        (ps pt : τ{bool})
        (itr_src : τ{codeT id_src_type st_src_type R_term})
-       (ktr_tgt : τ{(RV -> codeT id_tgt_type st_tgt_type R_term)%stype, δ + n}),
+       (ktr_tgt : τ{(RV -> codeT id_tgt_type st_tgt_type R_term)%stype, S (δ + n)}),
         (syn_triple_gen n δ tid P Q E ⊤ ps pt (trigger Yield;;; itr_src) code ktr_tgt))%S.
 
   Lemma red_syn_non_atomic_triple
         tid n δ (E : coPset)
-        (P : sProp (δ + n)) RV (code : itree tgtE RV) (Q : RV -> sProp (δ + n))
+        (P : sProp (S (δ + n))) RV (code : itree tgtE RV) (Q : RV -> sProp (S (δ + n)))
     :
-    ⟦syn_non_atomic_triple tid n δ E P code Q, δ + n⟧
+    ⟦syn_non_atomic_triple tid n δ E P code Q, S (δ + n)⟧
     =
-      non_atomic_triple tid (δ + n) n E ⟦P, δ + n⟧ code (fun v => ⟦Q v, δ + n⟧).
+      non_atomic_triple tid (S (δ + n)) n E ⟦P, S (δ + n)⟧ code (fun v => ⟦Q v, S (δ + n)⟧).
   Proof.
     unfold syn_non_atomic_triple, non_atomic_triple. red_tl.
     apply f_equal. extensionalities R_term. red_tl.
@@ -1495,7 +1495,7 @@ End TRIPLE.
 
 (* Triples. *)
 Notation "'[@' tid , n , E '@]' { P } code { v , Q }" :=
-  (syn_atomic_triple tid n 1 E P code (fun v => Q))
+  (syn_atomic_triple tid n 0 E P code (fun v => Q))
     (at level 200, tid, n, E, P, code, v, Q at level 1,
       format "[@  tid ,  n ,  E  @] { P }  code  { v ,  Q }") : sProp_scope.
 
@@ -1505,7 +1505,7 @@ Notation "'[@' tid , n , δ , E '@]' { P } code { v , Q }" :=
       format "[@  tid ,  n ,  δ ,  E  @] { P }  code  { v ,  Q }") : sProp_scope.
 
 Notation "'[@' tid , n , E '@]' ⧼ P ⧽ code ⧼ v , Q ⧽" :=
-  (syn_non_atomic_triple tid n 1 E P code (fun v => Q))
+  (syn_non_atomic_triple tid n 0 E P code (fun v => Q))
     (at level 200, tid, n, E, P, code, v, Q at level 1,
       format "[@  tid ,  n ,  E  @] ⧼ P ⧽  code  ⧼ v ,  Q ⧽") : sProp_scope.
 
