src/example/elimstack/ClientAdeqHOCAP.v
@@ -1,0 +1,242 @@
+From sflib Require Import sflib.
+From Paco Require Import paco.
+Require Import Coq.Classes.RelationClasses Lia Program.
+From Fairness Require Import pind Axioms ITreeLib Red TRed IRed2 WFLibLarge.
+From Fairness Require Import FairBeh Mod Concurrency Linking.
+From Fairness Require Import PCM IProp IPM IPropAux.
+From Fairness Require Import IndexedInvariants OpticsInterp SimWeakest SimWeakestAdequacy.
+From Fairness Require Import TemporalLogic SCMemSpec LifetimeRA AuthExclsRA ghost_excl ghost_map ghost_var.
+From Fairness.elimstack Require Import SpecHOCAP ClientCode ClientSpecHOCAP.
+From Fairness Require Export ModSim ModAdequacy ModCloseSim ModAddSim.
+From Fairness Require Export FIFOSched SchedSim FIFOSched FIFOSchedSim.
+
+Module ElimStackClientCorrect.
+
+  Definition config := [("thread_push", tt↑); ("thread_pop", tt↑)].
+
+  Notation src_state := (Mod.state ElimStackClientSpec.module).
+  Notation src_ident := (Mod.ident ElimStackClientSpec.module).
+  Notation tgt_state := (Mod.state ElimStackClient.module).
+  Notation tgt_ident := (Mod.ident ElimStackClient.module).
+
+  Local Instance STT : StateTypes := Build_StateTypes src_state tgt_state src_ident tgt_ident.
+
+  Local Instance Γ : SRA.t:=
+    GRA.of_list [
+        (* Default RAs. *)
+        OwnERA;
+        OwnDRA;
+        ThreadRA;
+        (stateSrcRA st_src_type);
+        (stateTgtRA st_tgt_type);
+        (identSrcRA id_src_type);
+        (identTgtRA id_tgt_type);
+        ObligationRA.t;
+        EdgeRA;
+        ArrowShotRA;
+        (* Additional RAs. *)
+        memRA;
+        Lifetime.t;
+        (AuthExcls.t (nat * nat));
+        (ghost_mapURA nat maybe_null_ptr);
+        (ghost_varURA (list SCMem.val));
+        (ghost_exclURA unit)
+      ].
+
+  (* Default RAs. *)
+  Local Instance _OWNERA : GRA.inG OwnERA Γ := (@GRA.InG _ Γ 0 (@eq_refl _ _)).
+  Local Instance _OWNDRA : GRA.inG OwnDRA Γ := (@GRA.InG _ Γ 1 (@eq_refl _ _)).
+  Local Instance _THDRA : GRA.inG ThreadRA Γ := (@GRA.InG _ Γ 2 (@eq_refl _ _)).
+  Local Instance _STATESRC : GRA.inG (stateSrcRA st_src_type) Γ := (@GRA.InG _ Γ 3 (@eq_refl _ _)).
+  Local Instance _STATETGT : GRA.inG (stateTgtRA st_tgt_type) Γ := (@GRA.InG _ Γ 4 (@eq_refl _ _)).
+  Local Instance _IDENTSRC : GRA.inG (identSrcRA id_src_type) Γ := (@GRA.InG _ Γ 5 (@eq_refl _ _)).
+  Local Instance _IDENTTGT : GRA.inG (identTgtRA id_tgt_type) Γ := (@GRA.InG _ Γ 6 (@eq_refl _ _)).
+  Local Instance _OBLGRA : GRA.inG ObligationRA.t Γ := (@GRA.InG _ Γ 7 (@eq_refl _ _)).
+  Local Instance _EDGERA : GRA.inG EdgeRA Γ := (@GRA.InG _ Γ 8 (@eq_refl _ _)).
+  Local Instance _ARROWSHOTRA : GRA.inG ArrowShotRA Γ := (@GRA.InG _ Γ 9 (@eq_refl _ _)).
+  Local Instance HasMemRA : GRA.inG memRA Γ := (@GRA.InG _ Γ 10 (@eq_refl _ _)).
+  Local Instance HasLifetime : GRA.inG Lifetime.t Γ := (@GRA.InG _ Γ 11 (@eq_refl _ _)).
+  Local Instance HasAuthExcls : GRA.inG (AuthExcls.t (nat * nat)) Γ := (@GRA.InG _ Γ 12 (@eq_refl _ _)).
+  Local Instance HasGhostMap : GRA.inG (ghost_mapURA nat maybe_null_ptr) Γ := (@GRA.InG _ Γ 13 (@eq_refl _ _)).
+  Local Instance HasGhostVar : GRA.inG (ghost_varURA (list SCMem.val)) Γ := (@GRA.InG _ Γ 14 (@eq_refl _ _)).
+  Local Instance HasGhostExcl : GRA.inG (ghost_exclURA unit) Γ := (@GRA.InG _ Γ 15 (@eq_refl _ _)).
+
+  Local Instance TLRASs : TLRAs_small STT Γ :=
+    @Build_TLRAs_small STT Γ _ _ _ _ _ _ _ _ _ _.
+
+  Local Instance Σ : GRA.t:=
+    GRA.of_list [
+        (* Default RAs. *)
+        OwnERA;
+        OwnDRA;
+        ThreadRA;
+        (stateSrcRA st_src_type);
+        (stateTgtRA st_tgt_type);
+        (identSrcRA id_src_type);
+        (identTgtRA id_tgt_type);
+        ObligationRA.t;
+        EdgeRA;
+        ArrowShotRA;
+        (* Additional RAs. *)
+        memRA;
+        Lifetime.t;
+        (AuthExcls.t (nat * nat));
+        (ghost_mapURA nat maybe_null_ptr);
+        (ghost_varURA (list SCMem.val));
+        (ghost_exclURA unit);
+        (* Maps from empty RAs of Γ. *)
+        (of_RA.t RA.empty);
+        (* Default RAs depending on sProp. *)
+        (IInvSetRA sProp);
+        (ArrowRA id_tgt_type (Vars:=sProp));
+        (ShareDutyRA id_tgt_type (Vars:=sProp))
+      ].
+
+  Local Program Instance sub : @SRA.subG Γ Σ :=
+    { subG_map := fun i => if (le_lt_dec i 15) then i else 16 }.
+  Next Obligation.
+    i. ss. unfold Σ, Γ. des_ifs.
+    - unfold GRA.of_list. simpl. des_ifs. all: lia.
+    - unfold GRA.of_list. simpl. des_ifs. all: lia.
+  Qed.
+
+  Local Instance _IINVSETRA : GRA.inG (IInvSetRA sProp) Σ := (@GRA.InG _ Σ 17 (@eq_refl _ _)).
+  Local Instance _ARROWRA : GRA.inG (ArrowRA id_tgt_type (Vars:=sProp)) Σ := (@GRA.InG _ Σ 18 (@eq_refl _ _)).
+  Local Instance _SHAREDUTY : GRA.inG (ShareDutyRA id_tgt_type (Vars:=sProp)) Σ := (@GRA.InG _ Σ 19 (@eq_refl _ _)).
+
+  Local Instance TLRAs : TLRAs STT Γ Σ :=
+    @Build_TLRAs STT Γ Σ _ _ _.
+
+  (* Additional initial resources. *)
+  Local Definition init_res :=
+    (GRA.embed (memory_init_resource ElimStackClient.gvs))
+      ⋅ (GRA.embed (AuthExcls.rest_ra (gt_dec 0) (0, 0))).
+
+  Arguments wpsim_bind_top {_ _ _ _ _ _}.
+  Arguments wpsim_wand {_ _ _ _ _ _}.
+  Arguments wpsim_ret {_ _ _ _ _ _}.
+
+  Ltac red_tl_all := red_tl; red_tl_memra; red_tl_lifetime; red_tl_authexcls.
+
+  Lemma correct:
+    UserSim.sim ElimStackClientSpec.module ElimStackClient.module
+                (prog2ths ElimStackClientSpec.module config) (prog2ths ElimStackClient.module config).
+  Proof.
+    eapply WSim.whole_sim_implies_usersim. econs.
+    { instantiate (1:=init_res). rr. splits.
+      { unfold init_res, default_initial_res. disj_tac. }
+      { ndtac. }
+      { unfold init_res. grawf_tac.
+        { apply memory_init_resource_wf. }
+        { ur. i. ur. split.
+          { rewrite URA.unit_idl. exists ε. rewrite URA.unit_id. auto. }
+          { ur. clarify. }
+        }
+      }
+    }
+    unfold init_res. repeat rewrite <- GRA.embed_add.
+    exists 3, 1. exists. lia.
+    eexists _. iIntros "(A & INIT)".
+    iDestruct (init_sat 0 1 with "[A INIT]") as "RES"; [ss| |].
+    { simpl. iFrame. iDestruct "A" as "[A B]". iSplitL "A"; iFrame. }
+
+    iEval (rewrite red_syn_fairI) in "RES". simpl. iMod "RES".
+    iDestruct "RES" as (?????) "(TGTST & #IsT & #CInv & Tpush & Dpush & Pc_kt_push & Pc_k_push & live_k & #Act_k & Tok & Pc_kt_pop & Tpop & Dpop)".
+    iEval (rewrite red_syn_tgt_interp_as) in "TGTST".
+    iDestruct "TGTST" as "#TGTST".
+    red_tl. simpl.
+
+    iModIntro. unfold natmap_prop_sum. ss.
+    iSplitR "Tpop Dpop Pc_kt_pop Tok".
+    { iDestruct (ElimStackClient_push_sim) as "RES".
+      iEval (red_tl) in "RES". iSpecialize ("RES" $! γk).
+      iEval (red_tl) in "RES". iSpecialize ("RES" $! kt).
+      iEval (red_tl) in "RES". iSpecialize ("RES" $! k).
+      iEval (red_tl) in "RES". iSpecialize ("RES" $! γs).
+      iEval (red_tl) in "RES". iSpecialize ("RES" $! γpop).
+      red_tl_all. simpl.
+      iEval (rewrite red_syn_wpsim) in "RES". iApply ("RES" with "[-]").
+      red_tl_all.
+      rewrite red_syn_tgt_interp_as. iFrame "∗#".
+    }
+    iSplit; [|done].
+    { iDestruct (ElimStackClient_pop_sim) as "RES".
+      iEval (red_tl) in "RES". iSpecialize ("RES" $! γk).
+      iEval (red_tl) in "RES". iSpecialize ("RES" $! k).
+      iEval (red_tl) in "RES". iSpecialize ("RES" $! kt).
+      iEval (red_tl) in "RES". iSpecialize ("RES" $! γs).
+      iEval (red_tl) in "RES". iSpecialize ("RES" $! γpop).
+      simpl. red_tl_all.
+      iEval (rewrite red_syn_wpsim) in "RES". iApply ("RES" with "[-]").
+      rewrite red_syn_tgt_interp_as. red_tl. red_tl_ghost_excl_ura. iFrame "∗#".
+    }
+  Qed.
+
+End ElimStackClientCorrect.
+
+Section ALL.
+
+  Definition client := ElimStackClient.module.
+  Definition client_spec := ElimStackClientSpec.module.
+
+  Lemma client_all_aux
+    :
+    Adequacy.improves
+      (interp_all
+         (client_spec.(Mod.st_init))
+         (prog2ths client_spec [("thread_push", tt↑); ("thread_pop", tt↑)]) 0)
+      (interp_all_fifo
+         (client.(Mod.st_init))
+         (prog2ths client [("thread_push", tt↑); ("thread_pop", tt↑)]) 0)
+  .
+  Proof.
+    eapply Adequacy.improves_trans.
+    { eapply Adequacy.adequacy.
+      { instantiate (1:=nat_wf). econs. exact 0. }
+      { i. ss. eauto. }
+      { eapply ssim_implies_gsim; ss.
+        { instantiate (1:=id). ss. }
+        { eapply ssim_nondet_fifo; ss. ii. compute in H. des. inv H; des; ss. inv H1; ss. }
+      }
+    }
+    eapply usersim_adequacy. eapply ElimStackClientCorrect.correct.
+    Unshelve. all: constructor.
+  Qed.
+
+  Theorem client_all
+    :
+    Adequacy.improves
+      (interp_concurrency
+         (prog2ths client_spec [("thread_push", tt↑); ("thread_pop", tt↑)])
+         (sched_nondet _)
+         (client_spec.(Mod.st_init))
+      )
+      (interp_concurrency
+         (prog2ths client [("thread_push", tt↑); ("thread_pop", tt↑)])
+         (sched_fifo_set _)
+         (client.(Mod.st_init))
+      )
+  .
+  Proof.
+    eapply client_all_aux.
+  Qed.
+
+  Theorem client_fair_sched
+    :
+    Adequacy.improves
+      (interp_concurrency
+         (prog2ths client_spec [("thread_push", tt↑); ("thread_pop", tt↑)])
+         (sched_nondet _)
+         (client_spec.(Mod.st_init))
+      )
+      (interp_concurrency
+         (prog2ths client [("thread_push", tt↑); ("thread_pop", tt↑)])
+         (sched_nondet _)
+         (client.(Mod.st_init))
+      )
+  .
+  Proof.
+    eapply usersim_adequacy. eapply ElimStackClientCorrect.correct.
+  Qed.
+
+End ALL.
